
>[!text]
>Cho hai ánh xạ: ${f : X \rightarrow Y}$ và ${g : Y \rightarrow Z}$. Ánh xạ ${h : X \rightarrow Z}$ được gọi là tích của hai ánh xạ $f$ và $g$

- Kí hiệu: ${g \circ f}$ 
- Ta có: ${g \circ f = g[f(x)], \forall x \in X}$

- Ví dụ:
>Cho ${f: \mathbb R \rightarrow \mathbb R}$ và ${g: \mathbb R \rightarrow \mathbb R}$ xác định bởi ${f(x) = 5x + 3}$ và ${g(x) = x^2 + 1}$
>Khi đó:
>${g \circ f(x) = (5x+3)^2 +1}$
>${f\circ g(x) = 5(x^2 + 1) + 3}$

- Từ đó có thể thấy ${g \circ f(x) \neq f \circ g(x)}$






